theories/check.v
@@ -377,9 +377,12 @@ Section check.
       have [[??]sD]:= expand_solved_same _ X; subst.
       have [[??]sB]:= expand_solved_same _ Y; subst.
       move=> s2 B b H3.
-      have [A'[B0'[B'[b1[b2[sm [?[[H4 H5]|[A''[H4[H5 H6]]]]]]]]]]] := run_and_correct_success_left _ sD H3; subst.
-        apply: H2 H4.
-      apply: H1 H4.
+      have:= runb_same_structure _ H3.
+      case: B H3 => //= ??? H3 _.
+      have [A''[b1[b2[sm[Hz[+ Hr]]]]]] := run_and_correct _ H3; subst.
+      case: ifP => Ht Hs.
+        apply: H1 Hz.
+      apply: H2 Hs.
   Qed.
 
   Lemma expandedb_next_alt_done {sP s A s1 B b}: 
@@ -407,8 +410,8 @@ Section check.
       by rewrite fun_if/=kA kB !is_ko_clean_success//kA kB if_same.
     - move=> A HA B0 _ B HB; rewrite fun_if/=.
       move=> /orP[H|/andP[H1 H2]].
-        rewrite H if_same//.
-      by rewrite HB H2//H1 if_same orbT.
+        rewrite H/= HA// if_same//.
+      rewrite HB H2//H1 !orbT if_same//.
   Qed.
 
   Lemma has_cut_next_alt {A B}: 
@@ -454,11 +457,11 @@ Section check.
       rewrite fun_if/=cA H1 HA//= is_ko_clean_success ?is_ko_cutr// cutr2 eqxx.
       by rewrite no_alt_cut !if_same.
     - move=> A HA B0 _ B HB /orP[kA|/and3P[H1 H2 H3]].
-        by rewrite fun_if/= kA if_same.
+        rewrite fun_if/= kA /= is_ko_clean_success// kA if_same//.
       rewrite fun_if/= H3 H2/= H1 orbT HB// !andbT.
       move: H1 => /orP[/andP[H4 H5]|H5].
         by rewrite H4 has_cut_clean_success//?orbT if_same.
-      by rewrite H5 !orbT if_same.
+      rewrite HA// !orbT if_same//.
   Qed.
 
   Lemma no_free_alt_next_alt {sP A B}:
